refocusing_signatures.v
@@ -14,19 +14,19 @@ Module Type RED_SEM (R : RED_LANG).
 
   Axiom decompose : forall (t : term) k1, ~ dead_ckind k1 ->
       (exists (v : value k1), t = v) \/
-      (exists k2 (r : redex k2) (c : context k1 k2), plug r c = t).
+      (exists k2 (r : redex k2) (c : context k1 k2), c[r] = t).
 
   (** dec is left inverse of plug *)
   Axiom dec_correct  : forall t {k1 k2} (c : context k1 k2) d, dec t c d -> 
-                           decomp_to_term d = plug t c.
+                           decomp_to_term d = c[t].
 
   Axiom dec_plug     : forall {k1 k2} (c : context k1 k2) {k3} (c0 : context k3 k1) t d, 
-                           ~ dead_ckind k2 -> dec (plug t c) c0 d -> 
+                           ~ dead_ckind k2 -> dec c[t] c0 d -> 
                            dec t (c ~+ c0) d.
 
   Axiom dec_plug_rev : forall {k1 k2} (c : context k1 k2) {k3} (c0 : context k3 k1) t d, 
                            ~ dead_ckind k2 ->  dec t (c ~+ c0) d -> 
-                           dec (plug t c) c0 d.
+                           dec c[t] c0 d.
 
   Inductive decempty : term -> forall {k}, decomp k -> Prop :=
   | d_intro : forall t {k} (d : decomp k), dec t [_] d -> decempty t d.
@@ -34,7 +34,7 @@ Module Type RED_SEM (R : RED_LANG).
   Inductive iter : forall {k}, decomp k -> value k -> Prop :=
   | i_val : forall {k} (v : value k), iter (d_val v) v
   | i_red : forall {k2} (r : redex k2) t {k1} (c : context k1 k2) d v,
-              contract r = Some t -> decempty (plug t c) d -> iter d v ->
+              contract r = Some t -> decempty c[t] d -> iter d v ->
               iter (d_red r c) v.
 
   Inductive eval : term -> forall {k}, value k -> Prop :=
@@ -58,16 +58,16 @@ Module Type RED_REF_SEM (R : RED_LANG).
       ~ dead_ckind (ckind_trans k ec0).*)
 
   Axiom dec_term_correct : forall t k, match dec_term t k with
-    | in_red r       => redex_to_term r = t
-    | in_val v       => value_to_term v = t
-    | in_term t0 ec0 => atom_plug t0 ec0 = t
+    | in_red r       => t = r
+    | in_val v       => t = v
+    | in_term t0 ec0 => t = ec0:[t0]
     | in_dead        => dead_ckind k
   end.
 
   Axiom dec_context_correct : forall ec k v, match dec_context ec k v with
-    | in_red r      => redex_to_term r = atom_plug v ec
-    | in_val v0     => value_to_term v0 = atom_plug (value_to_term v) ec
-    | in_term t ec0 => atom_plug t ec0 = atom_plug (value_to_term v) ec
+    | in_red r      => ec:[v] = r
+    | in_val v0     => ec:[v] = v0
+    | in_term t ec0 => ec:[v] = ec0:[t]
     | in_dead       => dead_ckind (k+>ec) 
   end.
 
@@ -83,7 +83,7 @@ Module Type RED_REF_SEM (R : RED_LANG).
                dec t c d
   | d_term : forall t t0 {k1 k2} (c : context k1 k2) ec d,
                dec_term t k2 = in_term t0 ec ->
-               dec t0 (ccons ec c) d ->
+               dec t0 (ec=:c) d ->
                dec t c d
   with decctx : forall {k2}, value k2 -> forall {k1}, context k1 k2 -> decomp k1 -> Prop :=
   | dc_end  : forall {k} (v : value k), 
@@ -91,17 +91,17 @@ Module Type RED_REF_SEM (R : RED_LANG).
                 decctx v [_] (d_val v)
   | dc_dec  : forall ec {k2} (v : value (k2+>ec)) {k1} (c : context k1 k2) r,
                 dec_context ec k2 v = in_red r ->
-                decctx v (ccons ec c) (d_red r c)
+                decctx v (ec=:c) (d_red r c)
   | dc_val  : forall {k2} (v0 : value k2) ec (v : value (k2+>ec)) 
                      {k1} (c  : context k1 k2) d,
                 dec_context ec k2 v = in_val v0 ->
                 decctx v0 c d ->
-                decctx v (ccons ec c) d
+                decctx v (ec=:c) d
   | dc_term : forall ec ec0 {k2} (v : value (k2+>ec)) 
                             {k1} (c : context k1 k2) t d,
                 dec_context ec k2 v = in_term t ec0 ->
-                dec t (ccons ec0 c) d ->
-                decctx v (ccons ec c) d.
+                dec t (ec0=:c) d ->
+                decctx v (ec=:c) d.
 
   Scheme dec_Ind := Induction for dec Sort Prop
    with decctx_Ind := Induction for decctx Sort Prop.
@@ -150,8 +150,8 @@ Module Type RED_SEM_PROPER (R : RED_LANG) (RS : RED_SEM R).
 
          (exists v : R.value k1, value_to_term v = t) \/
 
-         (exists k2 (r : redex k2) (c : context k1 k2), plug r c = t /\ 
+         (exists k2 (r : redex k2) (c : context k1 k2), c[r] = t /\ 
 	      forall k2' (r' : redex k2') (c' : context k1 k2'), 
-                  plug r' c' = t -> k2' = k2 /\ r ~= r' /\ c ~= c').
+                  c'[r'] = t -> k2' = k2 /\ r ~= r' /\ c ~= c').
 
 End RED_SEM_PROPER.
